---
title: "lecture 3 presentation"
author:
- \emph{Simon Fløj Thomsen}^[Aalborg University, sft@business.aau.dk, lokale 24 fib 11, MaMTEP] 
date: \emph{`r format(Sys.time(), '%B %d, %Y')`}
output:
  beamer_presentation: 
    toc: true
    slide_level: 2 
    theme: "AnnArbor"
    colortheme: "dolphin"
    fonttheme: "structurebold"
    
---


# Geometric series


## Geometriske serier review - Eksempler på serier

### Eksempel 1:

$$\sum^n_{n=1} x^n=x + x^2 + x^3 + x^4 +...+x^{n-1}$$


### Eksempel 2:

$$x + \sqrt{x} + 1 + \frac{1}{\sqrt{x}} + \frac{1}{x} ... $$

## Typer af geometriske serier

### Endelig serie

$\sum^n_{n=1} ak^n = a* \frac{1-k^n}{1-k}$,   $k \neq1$

### Uendelig serie

$\sum^n_{n=1} ak^n = \frac{a}{1-k}$,   $\lvert k \rvert  <1$


$\sum^n_{n=1} ak^n = na$,   $\lvert k \rvert  =1$



## Udregning

### Endelig serie

$$S_n = \alpha + \alpha*k + \alpha*k^2 + \alpha*k^3 + ... + \alpha*k^{n-1}$$
$$k*S_n = \alpha*k + \alpha*k^2 + \alpha*k^3 + \alpha*k^4 + ... + \alpha*k^{n}$$

$$S_n - k*S_n = \alpha + (\alpha*k - \alpha*k) + (\alpha*k^2- \alpha*k^2) + ... + (\alpha*k^{n-1} - \alpha*k^{n-1}) - \alpha*k^{n}$$

$$S_n - k*S_n = \alpha - \alpha*k^{n}$$

$$S_n(1-k) = \alpha(1-k^n)$$

$$S_n = \alpha * \frac{1-k^n}{1-k}$$

## Udregning

### Uendelig serie

Hvis $\vert k \vert <  1$ når $n \to \infty$ vil udtrykket gå mod:

$$S_n = \alpha * \frac{1}{1-k}$$

Dermed kan vi skrive:

$$ \sum_{n=1}^\infty = \frac{ \alpha}{1-k}$$

# Difference equations


## Math to econometrics

Today we will look at 1. order difference equations

In 2. semester math seen like this: 

$$x_t = ax_{t-1} + b$$
In time series econometrics you will see it like this, called an AR(1) process: 

$$y_t= \mu + \theta y_{t-1} + \varepsilon_t$$
We will look at what differences between these two equations

Lets first see what they got in common:

- Both equations got a constant $\mu$ and $b$

- Both equations got a coefficient $\theta$ and $a$

- Both equations got a variable that changes over time (discrete) $y_t$ and $x_t$


## Math to econometrics

The difference between the two equations is that in econometrics we got the error term $\varepsilon_t$ with the diffenition:

$$\varepsilon_t \sim IID(0,\sigma^2)$$
Explain! 

Later we take a look at how this changes things!


## Differens equations (Math)

Lets look at the difference equation again:

$$x_t = ax_{t-1} + b_t$$
We can start from a given point $x_0$ 

$$x_1 = ax_0 + b_1$$
$$x_2 = ax_1 + b_2 = a(ax_0 + b_1) + b_2 = a^2 x_0 + ab_1 + b_2$$
$$x_3 = ax_2 + b_3 = a(a^2x_0 + ab_1 + b_2) + b_3 = a^3x_0 + a^2 b_1 + ab_2 + b_3$$

## Differens equations (Math)

We can already see the pattern:

$$x_t= a^t x_0 + \sum^t_{k=1} a^{t-k} b_k$$

We now assume the case when $b_k = b$ so we now got a constant as in the AR(1) model.

So we can now write the last term as:

$$\sum^t_{k=1}a^{t-k}b$$ 
Which is a geometric series! that we just covered!

$$\sum^t_{k=1}a^{t-k}b= b(a^{t-1} + a^{t-2} + a^{t-3} +...+a +1) =\frac{(b-ba^t)}{(1-a)}$$

## Differens equations (Math)

Therefor we can now write: 

$$x_t= a^t (x_0 - \frac{b}{1-a}) + \frac{b}{1-a}$$

We can see that if $x_0 = \frac{b}{1-a}$ we get that $x_t= \frac{b}{1-a}$ which I have illustrated down below:

```{r, echo=FALSE}
knitr::include_graphics(rep("diff..png", 1), dpi = 300)
```


## Differens equations (Math)

In fact if just $x_s$ at any point hits $\frac{b}{1-a}$ we wont get away from it as:

$$x_{s+1} = a\frac{b}{1-a} +b = \frac{b}{1-a}$$

```{r, echo=FALSE}
knitr::include_graphics(rep("diff2.png", 1), dpi = 300)
```

But what if we never hit that value?

## Difference equations (stability)

### Case 1

$$\vert a \vert < 1$$
We then see that $a^t$ goes towards 0 as $t \to \infty$ in: 

$$x_t= a^t (x_0 - \frac{b}{1-a}) + \frac{b}{1-a}$$
And we will end up with 

$$x_t= \frac{b}{1-a}$$

### Case 2

$$\vert a \vert > 1$$

We then see that $a^t$ goes towards $\infty$ as $t \to \infty$ in and will explode. 


**But what if x_0 start below and we hit the value it should just stop right? Eller er det umuligt vil den eksplodere ned af i stedet?**

## Difference equations (stability)

```{r, echo=FALSE}
knitr::include_graphics(rep("diff3.png", 1), dpi = 150)
```

## AR(1) model Econometrics

Lets look at the AR(1) process again:

$$y_t= \mu + \theta y_{t-1} + \varepsilon_t$$
Where the only difference was the error term: $\varepsilon_t$ lets see some examples and what the difference is


## AR(1) model Exonometrics

To give an example we use the model:
$$y_t= 5 +  0.5y_{t-1}+\varepsilon_t$$

### Simulering
```{r, echo=FALSE, fig.height= 3.5}
suppressPackageStartupMessages(library(forecast))
# Set up variables
set.seed(1234)
n <- 1000
x <- matrix(0,1000,1)
w <- rnorm(n)

# loop to create x
for (t in 2:n) x[t] <- 5+ 0.5 * x[t-1] + w[t]
plot(x,type='l', main = "X_t= 5 + 0.5*X_t-1 + u_t"); abline( h=10, col= "red")
```

We see the shocks from $\varepsilon_t$ does so we never stay in $\frac{b}{1-a}$ as we did with the difference equations before

## AR(1) model Exonometrics

$$y_t= 5 +  1.5y_{t-1}+\varepsilon_t$$

### Simulering

```{r, echo=FALSE, fig.height= 5}

# Set up variables
set.seed(1234)
n <- 1000
x <- matrix(0,1000,1)
w <- rnorm(n)

# loop to create x
for (t in 2:n) x[t] <- 5+ 1.5 * x[t-1] + w[t]
plot(x,type='l', main = "X_t= 5 + 1.5*X_t-1 + u_t")

```


## AR(1) model Exonometrics

$$y_t= 5 +  1y_{t-1}+\varepsilon_t$$

### Simulering

```{r, echo=FALSE, fig.height= 5}
# Set up variables
set.seed(1234)
n <- 1000
x <- matrix(0,1000,1)
w <- rnorm(n)

# loop to create x
for (t in 2:n) x[t] <- 5+ 1 * x[t-1] + w[t]
plot(x,type='l', main = "X_t= 5 + 1*X_t-1 + u_t")
```


## AR(1) model Exonometrics (mean)

We saw before that we never stay the value $\frac{b}{1-a}$ in the AR(1) model, but what if we calculate the mean?

$$E[y_t] = E[\mu + \theta y_{t-1} + \varepsilon_t]$$
$$= \mu + \theta E[y_{t-1}] + E[\varepsilon]$$
$$= \mu + \theta E[\mu + \theta y_{t-2} + \varepsilon_{t-1}]$$
$$= \mu + \mu\theta+  \theta^2 E[y_{t-2}]$$
$$= \mu + \mu\theta+  \theta^2 E[\mu + \theta y_{t-3} + \varepsilon_{t-2}]$$
$$= \mu(1 + \theta + \theta^2 + \theta^3 + ... +\theta^\infty)$$


So back to the geometric series if $\vert \theta \vert< 1$ we get $\frac{\mu}{1-\theta}$


## AR(1) model Exonometrics (mean)

Lets try calculating the mean using the example from before before 

$$y_t= 5 +  0.5y_{t-1}+\varepsilon_t$$
$$E[y_t]= \frac{5}{1-0.5} = 10$$

Lets look at the plot again!

# Statistik opsumering


## Expected value

$$E(aX + b) = aE(X) + b$$
$$E(X+Y)= E(X)E(Y)$$

$$E(XY)= E(X)E(Y)$$

- Hvis X og Y er uafhæængige 

- Bevis for dette behøves i ik at kende 

## Variance 

$$Var(X) = E[X-E(X)]^2 = E(XX) - E(X)E(X)$$

- Vi kan se hvis $E(X)=0$ er $Var(X) = E(X^2)$

- Bevis ovenstående

$$Var(aX+b) = a^2 Var(X)$$
$$Var(X + Y) = Var(X) + Var(Y) + 2Cov(X,Y)$$

- Bevis ovenstående
$$Var(X + Y) = Var(X) + Var(Y)$$

- Hvis X og Y er uafhængige




## Bevis for Var(X)

$$Var(X) = E[X-E(X)]^2 = E(XX) - E(X)E(X)$$


- Løs på tavlen 


## Bevis for Var(X+Y)


$$Var(X+Y) = Var(X) + Var(Y) + 2Cov(X,Y)$$


## Covariance 

$$Cov(X,Y) = E[X-E(X)][Y-E(Y)]= E(XY) - E(X)E(Y)$$

- Bevis ovenstående

$$Cov(X,X) = Var(X)$$

$$Cov(aX + b, cY + d) = acCov(X,Y)$$

$$Cov(X + Y, Z) = Cov(X,Z) + Cov(Y,Z)$$



## Bevis Cov(X,Y)

$$Cov(X,Y) = E[X-E(X)][Y-E(Y)]= E(XY) - E(X)E(Y)$$

- Løs på tavlen


# Moving Average process opsumering: 


$$Y_t = \mu + \varepsilon_t + \alpha \varepsilon_{t-1}$$

$$\varepsilon_t \sim IID(0, \sigma^2)$$

- Calculate mean of $Y_t$

$$E[Y_t] = E[\mu]  E[\varepsilon_t] + E[\alpha \varepsilon_{t-1}]$$

- Vi ved $E[\varepsilon_t] = E[\varepsilon_{t-1}] = 0$

$$E[Y_t] = \mu$$

